isa/Gencot_ESArray_Lemmas.thy
@@ -1,0 +1,149 @@
+theory Gencot_ESArray_Lemmas
+  imports "Gencot_ESArray_Tuples"
+    "Gencot_CArray_Lemmas"
+begin
+
+text \<open>Extend the overloaded abstract data type to explicitly sized arrays.
+      Additionally introduce the following function for filling an array 
+      with an explicitly specified size.\<close>
+consts 
+  arr_fill_n :: "nat \<Rightarrow> (nat \<Rightarrow> 'el) \<Rightarrow> 'arr"
+
+text \<open>Define the abstract data type functions for explicitly sized arrays.
+The explicit size is ignored and the intrinsic size of the list is used.\<close>
+definition sizES :: "'el CArrES\<^sub>T \<Rightarrow> nat"
+  where "sizES a \<equiv> length (fst a)"
+definition vldES :: "'el CArrES\<^sub>T \<Rightarrow> nat \<Rightarrow> bool"
+  where "vldES a i \<equiv> i < sizES a"
+definition elmES :: "nat \<Rightarrow> 'el CArrES\<^sub>T \<Rightarrow> 'el"
+  where "elmES i a \<equiv> nth (fst a) i"
+definition elm_updateES :: "nat \<Rightarrow> ('el \<Rightarrow> 'el) \<Rightarrow> 'el CArrES\<^sub>T \<Rightarrow> 'el CArrES\<^sub>T"
+  where "elm_updateES i f a \<equiv> ((list_update (fst a) i (f (elmES i a))),snd a)"
+definition elm_modifiedES :: "nat \<Rightarrow> ('el \<Rightarrow> 'el \<Rightarrow> bool) \<Rightarrow> 'el CArrES\<^sub>T \<Rightarrow> 'el CArrES\<^sub>T \<Rightarrow> bool"
+  where elm_modified_def: "elm_modifiedES i m a1 a2 \<equiv> 
+    m (elmES i a1) (elmES i a2) \<and> (\<forall>j \<noteq> i. vldES a1 j \<longrightarrow> elmES j a1 = elmES j a2)"
+definition arr_fill_nES :: "nat \<Rightarrow> (nat \<Rightarrow> 'el) \<Rightarrow> 'el CArrES\<^sub>T"
+  where "arr_fill_nES n f \<equiv> ([f x . x \<leftarrow> [0 ..< n]],of_nat n)"
+
+text \<open>Laws for the abstract data type functions\<close>
+lemma vldArrES: "vldES a n = (n < length (fst a))"
+  by (simp add: vldES_def sizES_def)
+lemma elm_identUpdES[simp]: "elm_updateES i (\<lambda>a. a) = (\<lambda>a. a)"
+  apply (unfold elm_updateES_def)
+  by(simp add: elmES_def)
+lemma elm_sameUpdES: "elm_updateES i (\<lambda>_. m (elmES i x)) x = elm_updateES i m x"
+  by(simp add: elm_updateES_def)
+thm list_update_same_conv
+lemma elm_distUpdES: "vldES a i \<Longrightarrow> (elm_updateES i f) ( (elm_updateES i g) a) = elm_updateES i (f \<circ> g) a"
+  for f:: "'el \<Rightarrow> 'el" and a::"'el CArrES\<^sub>T"
+  apply (unfold elm_updateES_def elmES_def fst_def vldArrES)
+  by(auto)
+lemma elm_commUpd_elmES: "i < j \<Longrightarrow> (elm_updateES j m2) \<circ> (elm_updateES i m1) = (elm_updateES i m1) \<circ> (elm_updateES j m2)"
+  apply (unfold elm_updateES_def elmES_def)
+  apply(rule ext,simp)
+  apply(rule list_update_swap)
+  by(simp)
+lemma elmElmUpdES: "vldES a i \<Longrightarrow> elmES i (elm_updateES i f a) = f (elmES i a)"
+  by(auto simp add: elm_updateES_def elmES_def vldArrES)
+lemma elmElmUpdFrameES: "vldES a i \<and> vldES a j \<and> i \<noteq> j \<Longrightarrow> elmES j (elm_updateES i f a) = elmES j a"
+  by(auto simp add: elm_updateES_def elmES_def vldArrES)
+lemma elmArrFillES: "i < n \<Longrightarrow> elmES i (arr_fill_nES n f) = f i"
+  by(auto simp add: elmES_def arr_fill_nES_def vldArrES)
+
+text \<open>Array equality by extensionality. \<close>
+lemma eqArrES: "snd a1 = snd a2 \<Longrightarrow> sizES a1 = sizES a2 \<Longrightarrow>
+              (a1 = a2) = 
+              (\<forall> i. (vldES a1 i) \<longrightarrow> ((elmES i a1) = (elmES i a2)))"
+  for a1::"'el CArrES\<^sub>T" and a2::"'el CArrES\<^sub>T"
+  apply(rule iffI)
+   apply(rule allI)
+   apply(rule impI)
+   apply(auto simp add: elmES_def vldArrES sizES_def)
+  apply(case_tac a1)
+  apply(case_tac a2)
+  apply(auto)
+  apply(rule nth_equalityI)
+  by(auto)
+
+lemma eqElmUpdES: "sizES a1 = sizES a2 \<Longrightarrow> snd a1 = snd a2 \<Longrightarrow> vldES a2 i \<Longrightarrow> (a1 = elm_updateES i f a2) =
+                 ((elmES i a1) = f (elmES i a2) \<and> (\<forall> j. j \<noteq> i \<and> (vldES a1 j) \<longrightarrow> (elmES j a1) = (elmES j a2)))"
+  apply(rule iffI)
+   apply(auto)
+    apply(subst elmElmUpdES,auto)
+  apply(subst elmElmUpdFrameES,auto simp add: vldArrES sizES_def)
+  apply(subst eqArrES)
+    apply(auto simp add:elm_updateES_def)
+   apply(auto simp add: sizES_def)
+   apply(auto simp add: elmES_def)
+  apply(case_tac "ia = i")
+   apply(simp)
+  by(auto simp add: vldArrES)
+lemma eqArrFillES: "sizES a = n \<Longrightarrow> snd a = of_nat n \<Longrightarrow> (a = arr_fill_nES n f) = 
+                 ((\<forall> i. (vldES a i) \<longrightarrow> ((elmES i a) = f i)))"
+  apply(rule iffI)
+   apply(auto)
+   apply(rule elmArrFillES)
+   apply(simp add: vldArrES arr_fill_nES_def)
+  apply(subst eqArrES)
+   apply(simp add: vldArrES arr_fill_nES_def)
+   apply(simp add: sizES_def arr_fill_nES_def)
+   apply(rule allI)
+   apply(rule impI)
+  apply(subst elmArrFillES)
+  by (auto simp add: vldArrES sizES_def)
+
+text \<open>Semantics theorems for the Gencot array functions.\<close>
+
+definition ctrct_getArrES :: "'el CArrES\<^sub>T \<times> ('m::len) word \<Rightarrow> bool"
+  where ctrct_getArrES_def[simp]:
+  "ctrct_getArrES x \<equiv> let ((a,n),i) = x in unat n = length a \<and> (unat i) < (unat n)"
+theorem sem_getArrES[sem]: 
+ "ctrct_getArrES (a,i) \<Longrightarrow> 
+  getArrES (a,i) = elmES (unat i) a"
+  by (auto simp add: getArrES_def elmES_def)
+
+definition ctrct_setArrES :: "'el CArrES\<^sub>T \<times> ('m::len) word \<times> 'el \<Rightarrow> bool"
+  where ctrct_setArrES_def[simp]:
+  "ctrct_setArrES x \<equiv> let ((a,n),i,v) = x in unat n = length a \<and> (unat i) < (unat n)"
+theorem sem_setArrES[sem]: 
+ "ctrct_setArrES (a,i,v) \<Longrightarrow> 
+  setArrES (a,i,v) = (elm_updateES (unat i) (\<lambda>_.v) a, ())"
+  by (auto simp add: setArrES_def elm_updateES_def)
+
+definition ctrct_modifyArrES :: "'el CArrES\<^sub>T \<times> ('m::len) word \<times> ('el \<times> 'arg \<Rightarrow> 'el \<times> 'arg) \<times> 'arg \<Rightarrow> bool"
+  where ctrct_modifyArrES_def[simp]:
+  "ctrct_modifyArrES x \<equiv> let ((a,n),i,f,v) = x in unat n = length a \<and> (unat i) < (unat n)"
+theorem sem_modifyArrES[sem]:
+ "ctrct_modifyArrES (a,i,f,x) \<Longrightarrow> 
+  modifyArrES (a,i,f,x) = 
+  (let (e,y) = f (elmES (unat i) a, x) in (elm_updateES (unat i) (\<lambda>_.e) a, y))"
+  by (simp add: modifyArrES_def split_def Let_def elm_updateES_def elmES_def)
+
+definition ctrct_modifyArrDfltES :: "'el CArrES\<^sub>T \<times> ('m::len) word \<times> ('el \<times> 'arg \<Rightarrow> 'el \<times> 'out) \<times> 'arg \<Rightarrow> bool"
+  where ctrct_modifyArrDfltES_def[simp]:
+  "ctrct_modifyArrDfltES x \<equiv> let ((a,n),i,f,v) = x in unat n = length a \<and> (unat i) < (unat n)"
+theorem sem_modifyArrDfltES[sem]:
+ "ctrct_modifyArrDfltES (a,i,f,x) ==> 
+  modifyArrDfltES (a,i,f,x) = 
+  (let (e,y) = f (elmES (unat i) a, x) in (elm_updateES (unat i) (\<lambda>_.e) a, y))"
+  by (simp add: modifyArrDfltES_def split_def Let_def elm_updateES_def elmES_def)
+
+definition ctrct_modrefArrES :: "'el CArrES\<^sub>T \<times> ('m::len) word \<times> ('pel \<times> 'arg \<Rightarrow> 'pel \<times> 'arg) \<times> 'arg \<Rightarrow> bool"
+  where ctrct_modrefArrES_def[simp]:
+  "ctrct_modrefArrES x \<equiv> let ((a,n),i,f,v) = x in unat n = length a \<and> (unat i) < (unat n)"
+theorem sem_modrefArrES[sem]:
+ "ctrct_modrefArrES (a,i,f,x) \<Longrightarrow> 
+  modrefArrES (a,i,f,x) = 
+  (let (e,y) = f (toPtr (elmES (unat i) a), x) in (elm_updateES (unat i) (\<lambda>_.frPtr e) a, y))"
+  by (simp add: modrefArrES_def split_def Let_def elm_updateES_def elmES_def)
+
+definition ctrct_modrefArrDfltES :: "'el CArrES\<^sub>T \<times> ('m::len) word \<times> ('pel \<times> 'arg \<Rightarrow> 'pel \<times> 'out) \<times> 'arg \<Rightarrow> bool"
+  where ctrct_modrefArrDfltES_def[simp]:
+  "ctrct_modrefArrDfltES x \<equiv> let ((a,n),i,f,v) = x in unat n = length a \<and> (unat i) < (unat n)"
+theorem sem_modrefArrDfltES[sem]:
+ "ctrct_modrefArrDfltES (a,i,f,x) ==> 
+  modrefArrDfltES (a,i,f,x) = 
+  (let (e,y) = f (toPtr (elmES (unat i) a), x) in (elm_updateES (unat i) (\<lambda>_.frPtr e) a, y))"
+  by (simp add: modrefArrDfltES_def split_def Let_def elm_updateES_def elmES_def)
+
+end
